Replace undef_or_err with err_or_ub

src/coq/Utils/Error.v
@@ -10,8 +10,12 @@
 
 (* begin hide *)
 From Coq Require Import String.
-Require Import ExtLib.Structures.Monads.
-Require Export ExtLib.Data.Monads.EitherMonad.
+
+From ExtLib Require Import
+     Structures.Monads
+     Structures.Functor
+     Structures.MonadExc
+     Data.Monads.EitherMonad.
 
 From ITree Require Import
      ITree
@@ -65,36 +69,99 @@ Definition failwith {A:Type} {F} `{Monad F} `{MonadExc string F} (s:string) : F 
 #[export] Hint Unfold failwith: core.
 Arguments failwith _ _ _ _: simpl nomatch.
 
-(* SAZ:
-   I believe that these refer to "undefined behavior", not "undef" values.  
-   Raname them to "UB" and "UB_or_err"?
-   YZ: I agree 
-   TODO
-*)
-Definition undef := err.
-Definition undef_or_err := eitherT string err.
+Inductive UB_MESSAGE :=
+| UB_message : string -> UB_MESSAGE
+.
 
-Instance Monad_undef_or_err : Monad undef_or_err.
-unfold undef_or_err. typeclasses eauto.
+Inductive ERR_MESSAGE :=
+| ERR_message : string -> ERR_MESSAGE
+.
+
+Notation UB := (sum UB_MESSAGE).
+Notation ERR := (sum ERR_MESSAGE).
+
+Instance Exception_UB : MonadExc UB_MESSAGE UB := Exception_either UB_MESSAGE.
+Instance Exception_ERR : MonadExc ERR_MESSAGE ERR := Exception_either ERR_MESSAGE.
+
+Class VErrorM (M : Type -> Type) : Type :=
+  { raise_error : forall {A}, string -> M A }.
+
+Class UBM (M : Type -> Type) : Type :=
+  { raise_ub : forall {A}, string -> M A }.
+
+#[global] Instance VErrorM_E_MT {M : Type -> Type} {MT : (Type -> Type) -> Type -> Type} `{MonadT (MT M) M} `{VErrorM M} : VErrorM (MT M) :=
+  { raise_error := fun A e => lift (raise_error e);
+  }.
+
+#[global] Instance UBM_E_MT {M : Type -> Type} {MT : (Type -> Type) -> Type -> Type} `{MonadT (MT M) M} `{UBM M} : UBM (MT M) :=
+  { raise_ub := fun A e => lift (raise_ub e);
+  }.
+
+#[global] Instance VErrorM_MonadExc {M} `{MonadExc ERR_MESSAGE M} : VErrorM M
+  := { raise_error := fun _ msg => MonadExc.raise (ERR_message msg) }.
+
+#[global] Instance UBM_MonadExc {M} `{MonadExc UB_MESSAGE M} : UBM M
+  := { raise_ub := fun _ msg => MonadExc.raise (UB_message msg) }.
+
+Instance Exception_UB_string : MonadExc string UB :=
+  {| MonadExc.raise := fun _ msg => inl (UB_message msg);
+     catch := fun T c h =>
+                match c with
+                | inl (UB_message msg) => h msg
+                | inr _ => c
+                end
+  |}.
+
+Instance Exception_ERR_string : MonadExc string ERR :=
+  {| MonadExc.raise := fun _ msg => inl (ERR_message msg);
+     catch := fun T c h =>
+                match c with
+                | inl (ERR_message msg) => h msg
+                | inr _ => c
+                end
+  |}.
+
+Definition err_to_ERR {A} (e : err A) : ERR A
+  := match e with
+     | inl e => inl (ERR_message e)
+     | inr x => inr x
+     end.
+
+Definition lift_err {M A} `{MonadExc string M} `{Monad M} (e : err A) : (M A)
+  := match e with
+     | inl e => MonadExc.raise e
+     | inr x => ret x
+     end.
+
+Definition lift_ERR {M A} `{MonadExc ERR_MESSAGE M} `{Monad M} (e : ERR A) : (M A)
+  := match e with
+     | inl e => MonadExc.raise e
+     | inr x => ret x
+     end.
+
+Definition err_or_ub := eitherT ERR_MESSAGE UB.
+
+Instance Monad_err_or_ub : Monad err_or_ub.
+unfold err_or_ub. typeclasses eauto.
 Defined.
 
-Instance EqM_undef_or_err : Monad.Eq1 undef_or_err :=
-  fun (a : Type) (x y : undef_or_err a) => x = y.
+Instance EqM_err_or_ub : Monad.Eq1 err_or_ub :=
+  fun (a : Type) (x y : err_or_ub a) => x = y.
 
-Instance EqMProps_undef_or_err : Monad.Eq1Equivalence undef_or_err.
+Instance EqMProps_err_or_ub : Monad.Eq1Equivalence err_or_ub.
 constructor; intuition.
 repeat intro. etransitivity; eauto.
 Defined.
 
-Instance MonadLaws_undef_or_err: Monad.MonadLawsE undef_or_err.
+Instance MonadLaws_err_or_ub: Monad.MonadLawsE err_or_ub.
 constructor.
 - repeat intro. cbn. destruct (f x). cbn. reflexivity.
 - repeat intro. cbn. destruct x. cbn. destruct unEitherT; try reflexivity.
   destruct s; reflexivity.
-- repeat intro. cbn. destruct x. destruct unEitherT; destruct s; reflexivity.
+- repeat intro. cbn. destruct x. destruct unEitherT.
+  destruct u; destruct s; reflexivity.
+  destruct s; reflexivity.
 - repeat intro. destruct x, y. rewrite H. destruct unEitherT, unEitherT0; cbn; try reflexivity.
-  destruct s0; [reflexivity | rewrite H0; reflexivity].
+  destruct s; [reflexivity | rewrite H0; reflexivity].
   destruct s0; [reflexivity | rewrite H0; reflexivity].
 Qed.
-
-
